
The idea is clear : 

x1+x2+x3+...+xn=sum1.  y1+y2+y3+...yn=sum2.

So we can get :

① `(x1+x2+x3+...+xn)-(y1+y2+y3+...yn)=sum1-sum2;`

If we want to change x3 and y3,,then the equation will be :

② `(x1+x2+y3+...+xn)-(y1+y2+y3+...xn)=0`

use equation ① to minus equation ②：

`x3-y3+x3-y3=sum1-sum2` -> `x3-y3=(sum1-sum2)/2`

Solution 1. **Invalid** It cannot pass the last testcase

```Java
class Solution {
    public int[] findSwapValues(int[] array1, int[] array2) {
        int sum1=0,sum2=0;
        for(int item:array1)
            sum1+=item;
        for(int item:array2)
            sum2+=item;
        int gap=sum1-sum2;
        if(gap%2!=0)
            return new int[]{};
        gap/=2;
        for(int item1:array1) {
            for(int item2:array2) {
                if(item1-item2==gap)
                    return new int[]{item1,item2};
            }
        }

        return new int[]{};
        
    }
}

```

Solution 2. Somehow like two-sum , a trade-off between space complexity and time complexity

```Java

class Solution {
    public int[] findSwapValues(int[] array1, int[] array2) {
        Set<Integer> set = new HashSet<>();
        int sum1=0,sum2=0;
        for(int item:array1)
            sum1+=item;
        for(int item:array2) {
            sum2+=item;
            set.add(item);
        }
        int gap=sum1-sum2;
        if(gap%2!=0)
            return new int[]{};
        gap/=2;
        Arrays.sort(array1);
        Arrays.sort(array2);
       
        for(int item1:array1) {
            if(set.contains(item1-gap))
                return new int[]{item1,item1-gap};
        }

        return new int[]{};
        
    }
}

```